\documentclass[a4paper,12pt]{article}

\usepackage{graphicx}
\usepackage{amsmath}
\usepackage{tkz-euclide}

\begin{document}
\title{Assignment 8}
\author{Junaid Ahmad Bhat}
\date{January 25, 2021}
\maketitle

\section*{\small Question}
Express the matrix \begin{equation*}
B = 
\begin{pmatrix}
2 & -2 & -4 \\
-1 & 3 & 4 \\
1 & -2 & -3
\end{pmatrix}
\end{equation*}
as the sum of a symmetric and a skew symmetric matrix.\\

\section*{\small Solution}

We can write given matrix B as below:\\

B = $\dfrac{2B}{2}$ + (B'- B')     \hspace*{3cm}  (B' being transpose of B)\\

B = $\dfrac{B+B'}{2}$ + $\dfrac{B-B'}{2}$ \\

we have,
\begin{equation*}
B'=
\begin{pmatrix}
2 & -1 & 1 \\
-2 & 3 & -2 \\
-4 & 4 & -3
\end{pmatrix}
\end{equation*}\\

Let X =  $\dfrac{B+B'}{2}$ ; Y = $\dfrac{B-B'}{2}$\\

Therefore,
B = X + Y  \hspace*{3cm}(1)\\

\pagebreak

\textbf{let's evaluate X}:\\

2X = B + B'\\

 \hspace*{0.5cm}=  $\begin{pmatrix}2 & -2 & -4 \\-1 & 3 & 4 \\1 & -2 & -3\end{pmatrix} + \begin{pmatrix}2 & -1 & 1 \\-2 & 3 & -2 \\-4& 4& -3\end{pmatrix}$\\

\hspace*{1cm}

\hspace*{0.5cm}= $\begin{pmatrix}4 & -3 & -3 \\-3 & 6 & 2 \\-3 & 2 & -6\end{pmatrix}$\\

\hspace*{1cm}

 X = $\begin{pmatrix}2 & -3/2 & -3/2 \\-3/2 & 3 & 1 \\-3/2 & 1 & -3\end{pmatrix}$\\

and\\

 X' = $\begin{pmatrix}2 & -3/2 & -3/2 \\-3/2 & 3 & 1 \\-3/2 & 1 & -3\end{pmatrix}$ = X
 
\vspace*{1cm}
 
i,e X is symmetric matrix \hspace*{3cm}(as X'= X)\\

\hspace*{0.5cm}

\textbf{Similarly, evaluating Y}\\

2Y = B - B'\\

\hspace*{0.5cm}=  $\begin{pmatrix}2 & -2 & -4 \\-1 & 3 & 4 \\1 & -2 & -3\end{pmatrix} - \begin{pmatrix}2 & -1 & 1 \\-2 & 3 & -2 \\-4& 4& -3\end{pmatrix}$\\

\hspace*{1cm}

\hspace*{0.5cm}= $\begin{pmatrix}0 & -1 & -5 \\1 & 0 & 6 \\5 & -6 & 0\end{pmatrix}$\\

\hspace*{1cm}

Y = $\begin{pmatrix}0 & -1/2 & -5/2 \\1/2 & 0 & 3 \\5/2 & -3 & 0\end{pmatrix}$\\
 
and\\

Y' = $\begin{pmatrix}0 & 1/2 & 5/2 \\-1/2 & 0 & -3 \\-5/2 & 3 & 0\end{pmatrix}$ = -Y \\
\vspace*{1cm}

i,e Y is skew symmetric matrix \hspace*{3cm}(as Y'= -Y)\\
 
As B = X(symmetric) + Y(skew symmetric)  \hspace*{2cm} (by eqn (1))\\

$\Rightarrow \begin{pmatrix}2 & -2 & -4 \\-1 & 3 & 4 \\1 & -2 & -3\end{pmatrix}$ = $\begin{pmatrix}2 & -3/2 & -3/2 \\-3/2 & 3 & 1 \\-3/2 & 1 & -3\end{pmatrix}$ + $\begin{pmatrix}0 & -1/2 & -5/2 \\1/2 & 0 & 3 \\5/2 & -3 & 0\end{pmatrix}$\\

\vspace*{1cm}

Hence,it is decomposed/expressed as a sum of symmetric and skew symmetric matrix.

\pagebreak



 


\end{document}
